ocaml/ImpHConsOracles.mli
@@ -1,4 +1,5 @@
 open ImpPrelude
 open HConsingDefs
 
+val make_dict : 'a Dict.hash_params -> ('a, 'b) Dict.t
 val xhCons: 'a hashH -> 'a hashConsing
