ImpHCons.v
@@ -3,8 +3,6 @@ Require Export ImpIO.
 Import Notations.
 Local Open Scope impure.
 
-(********************************)
-(* (Weak) HConsing              *)
 
 Axiom string_of_hashcode: hashcode -> ?? caml_string.
 Extract Constant string_of_hashcode => "string_of_int".
@@ -12,7 +10,100 @@ Extract Constant string_of_hashcode => "string_of_int".
 Axiom hash: forall {A}, A -> ?? hashcode.
 Extract Constant hash => "Hashtbl.hash".
 
+(**************************)
+(* (Weak) Sets            *)
 
+
+Import Dict.
+
+Axiom make_dict: forall {A B}, (hash_params A) -> ?? Dict.t A B.
+Extract Constant make_dict => "ImpHConsOracles.make_dict".
+
+
+Module Sets.
+
+Definition t {A} (mod: A -> Prop) := Dict.t A {x | mod x}.
+
+Definition empty {A} (hp: hash_params A) {mod:A -> Prop}: ?? t mod :=
+  make_dict hp.
+
+Program Fixpoint add {A} (l: list A) {mod: A -> Prop} (d: t mod): forall {H:forall x, List.In x l -> mod x}, ?? unit :=
+  match l with
+  | nil => fun H => RET ()
+  | x::l' => fun H =>
+    d.(set)(x,x);;
+    add l' d
+  end.
+
+Program Definition create {A} (hp: hash_params A) (l:list A): ?? t (fun x => List.In x l) :=
+  DO d <~ empty hp (mod:=fun x => List.In x l);;
+  add l (mod:=fun x => List.In x l) d (H:=_);;
+  RET d.
+Global Opaque create.
+
+Definition is_present {A} (hp: hash_params A) (x:A) {mod} (d:t mod): ?? bool :=
+  DO oy <~ (d.(get)) x;;
+  match oy with
+  | Some y => hp.(test_eq) x (`y)
+  | None => RET false
+  end.
+
+Local Hint Resolve test_eq_correct: wlp.
+
+Lemma is_present_correct A (hp: hash_params A) x mod (d:t mod):
+ WHEN is_present hp x d ~> b THEN b=true -> mod x.
+Proof.
+  wlp_simplify; subst; eauto.
+  - apply proj2_sig.
+  - discriminate. 
+Qed.
+Hint Resolve is_present_correct: wlp.
+Global Opaque is_present.
+
+Definition msg_assert_incl: pstring := "Sets.assert_incl".
+
+Fixpoint assert_incl {A} (hp: hash_params A) (l: list A) {mod} (d:t mod): ?? unit :=
+  match l with
+  | nil => RET ()
+  | x::l' =>
+    DO b <~ is_present hp x d;;
+    if b then
+      assert_incl hp l' d
+    else (
+      hp.(log) x;;
+      FAILWITH msg_assert_incl
+    )
+  end.
+
+Lemma assert_incl_correct A (hp: hash_params A) l mod (d:t mod):
+ WHEN assert_incl hp l d ~> _ THEN forall x, List.In x l -> mod x.
+Proof.
+  induction l; wlp_simplify; subst; eauto.
+Qed.
+Hint Resolve assert_incl_correct: wlp.
+Global Opaque assert_incl.
+
+Definition assert_list_incl {A} (hp: hash_params A) (l1 l2: list A): ?? unit :=
+  (* println "";;print("dict_create ");;*)
+  DO d <~ create hp l2;;
+  (*print("assert_incl ");;*)
+  assert_incl hp l1 d.
+
+Lemma assert_list_incl_correct A (hp: hash_params A) l1 l2:
+ WHEN assert_list_incl hp l1 l2 ~> _ THEN List.incl l1 l2.
+Proof.
+  wlp_simplify.
+Qed.
+Global Opaque assert_list_incl.
+Hint Resolve assert_list_incl_correct.
+
+End Sets.
+
+
+
+
+(********************************)
+(* (Weak) HConsing              *)
 
 Module HConsing.
 
